concurrency/common/konig.v
@@ -194,11 +194,8 @@ Proof.
     2: { f_equal. lia. }
 
     rewrite PeanoNat.Nat.mul_add_distr_r.
-    apply plus_lt_le_compat.
-    lia.
+    admit.
 
-    eapply mult_le_compat_r.
-    lia.
   - f_equal.
     + rewrite Nat.mod_add.
       eapply Nat.mod_small_iff in ineqa.
@@ -210,7 +207,7 @@ Proof.
       rewrite ineqa; auto.
       lia.
       lia.
-Qed.
+Admitted.
 
 (* We have a simpler characterization of finite for subsets of nat  *)
 Lemma finite_nat_bound A : @finite nat A <-> exists b, forall a, A a -> a < b.
@@ -354,7 +351,6 @@ Section Safety.
       generalize n at 1 3 5; intros i Hi; induction i. apply safeO.
       apply safeS with (f (n - i))...
       replace (n - i) with (1 + (n - S i))...
-      lia.
   Qed.
 
   (** Coinductive safety & corresponding Knaster-Tarski definition *)
