concurrency/juicy/semax_safety_freelock.v
@@ -10,12 +10,19 @@ Require Import compcert.common.Values.
 
 Require Import VST.msl.Coqlib2.
 Require Import VST.msl.eq_dec.
+Require Import VST.msl.seplog.
+Require Import VST.msl.age_to.
+Require Import VST.veric.aging_lemmas.
+Require Import VST.veric.initial_world.
 Require Import VST.veric.juicy_mem.
 Require Import VST.veric.juicy_mem_lemmas.
 Require Import VST.veric.semax_prog.
+Require Import VST.veric.compcert_rmaps.
 Require Import VST.veric.Clight_core.
 Require Import VST.veric.Clightcore_coop.
 Require Import VST.veric.semax.
+Require Import VST.veric.semax_ext.
+Require Import VST.veric.juicy_extspec.
 Require Import VST.veric.juicy_safety.
 Require Import VST.veric.initial_world.
 Require Import VST.veric.juicy_extspec.
@@ -24,6 +31,7 @@ Require Import VST.veric.semax_ext.
 Require Import VST.veric.res_predicates.
 Require Import VST.veric.mem_lessdef.
 Require Import VST.veric.shares.
+Require Import VST.veric.age_to_resource_at.
 Require Import VST.floyd.coqlib3.
 Require Import VST.floyd.field_at.
 Require Import VST.sepcomp.step_lemmas.
@@ -38,7 +46,11 @@ Require Import VST.concurrency.common.addressFiniteMap.
 Require Import VST.concurrency.common.permissions.
 Require Import VST.concurrency.juicy.JuicyMachineModule.
 Require Import VST.concurrency.juicy.sync_preds_defs.
+Require Import VST.concurrency.juicy.sync_preds.
 Require Import VST.concurrency.juicy.join_lemmas.
+(*Require Import VST.concurrency.cl_step_lemmas.
+Require Import VST.concurrency.resource_decay_lemmas.
+Require Import VST.concurrency.resource_decay_join.*)
 Require Import VST.concurrency.juicy.semax_invariant.
 Require Import VST.concurrency.juicy.semax_simlemmas.
 Require Import VST.concurrency.juicy.sync_preds.
@@ -455,7 +467,7 @@ Proof.
     apply env_coherence_pures_eq with Phi; auto. lia.
     apply pures_same_pures_eq. auto.
     eapply rmap_freelock_pures_same; eauto.
-  - unfold ext_compat; rewrite age_to_ghost_of.
+  - rewrite age_to_ghost_of.
     destruct Hrmap' as (? & ? & ? & <-).
     destruct extcompat as [? J]; eapply ghost_fmap_join in J; eexists; eauto.
 
@@ -752,7 +764,7 @@ Proof.
       -- intros c' Ec'; specialize (safety c' Ec'). apply jsafe_phi_fupd_age_to; auto.
       -- destruct safety as (q_new & Einit & safety).
          exists q_new; split; auto.
-         apply jsafe_phi_fupd_age_to; auto.
+         apply jsafe_phi_age_to; auto.
     }
 
   - (* threads_wellformed *)
